src/ZF/UNITY/SubstAx.thy
@@ -1,24 +1,441 @@
-(*  Title:      ZF/UNITY/SubstAx.thy
-    ID:         $Id$
+(*  ID:         $Id$
     Author:     Sidi O Ehmety, Computer Laboratory
     Copyright   2001  University of Cambridge
-
-Weak LeadsTo relation (restricted to the set of reachable states)
 
 Theory ported from HOL.
 *)
 
-SubstAx = WFair + Constrains + 
+header{*Weak LeadsTo relation (restricted to the set of reachable states)*}
+
+theory SubstAx
+imports WFair Constrains 
+
+begin
 
 constdefs
   (* The definitions below are not `conventional', but yields simpler rules *)
-   Ensures :: "[i,i] => i"            (infixl 60)
+   Ensures :: "[i,i] => i"            (infixl "Ensures" 60)
     "A Ensures B == {F:program. F : (reachable(F) Int A) ensures (reachable(F) Int B) }"
 
-  LeadsTo :: "[i, i] => i"            (infixl 60)
+  LeadsTo :: "[i, i] => i"            (infixl "LeadsTo" 60)
     "A LeadsTo B == {F:program. F:(reachable(F) Int A) leadsTo (reachable(F) Int B)}"
 
 syntax (xsymbols)
-  "op LeadsTo" :: "[i, i] => i" (infixl " \\<longmapsto>w " 60)
+  "LeadsTo" :: "[i, i] => i" (infixl " \<longmapsto>w " 60)
+
+
+
+(*Resembles the previous definition of LeadsTo*)
+
+(* Equivalence with the HOL-like definition *)
+lemma LeadsTo_eq: 
+"st_set(B)==> A LeadsTo B = {F \<in> program. F:(reachable(F) Int A) leadsTo B}"
+apply (unfold LeadsTo_def)
+apply (blast dest: psp_stable2 leadsToD2 constrainsD2 intro: leadsTo_weaken)
+done
+
+lemma LeadsTo_type: "A LeadsTo B <=program"
+by (unfold LeadsTo_def, auto)
+
+(*** Specialized laws for handling invariants ***)
+
+(** Conjoining an Always property **)
+lemma Always_LeadsTo_pre: "F \<in> Always(I) ==> (F:(I Int A) LeadsTo A') <-> (F \<in> A LeadsTo A')"
+by (simp add: LeadsTo_def Always_eq_includes_reachable Int_absorb2 Int_assoc [symmetric] leadsToD2)
+
+lemma Always_LeadsTo_post: "F \<in> Always(I) ==> (F \<in> A LeadsTo (I Int A')) <-> (F \<in> A LeadsTo A')"
+apply (unfold LeadsTo_def)
+apply (simp add: Always_eq_includes_reachable Int_absorb2 Int_assoc [symmetric] leadsToD2)
+done
+
+(* Like 'Always_LeadsTo_pre RS iffD1', but with premises in the good order *)
+lemma Always_LeadsToI: "[| F \<in> Always(C); F \<in> (C Int A) LeadsTo A' |] ==> F \<in> A LeadsTo A'"
+by (blast intro: Always_LeadsTo_pre [THEN iffD1])
+
+(* Like 'Always_LeadsTo_post RS iffD2', but with premises in the good order *)
+lemma Always_LeadsToD: "[| F \<in> Always(C);  F \<in> A LeadsTo A' |] ==> F \<in> A LeadsTo (C Int A')"
+by (blast intro: Always_LeadsTo_post [THEN iffD2])
+
+(*** Introduction rules \<in> Basis, Trans, Union ***)
+
+lemma LeadsTo_Basis: "F \<in> A Ensures B ==> F \<in> A LeadsTo B"
+by (auto simp add: Ensures_def LeadsTo_def)
+
+lemma LeadsTo_Trans:
+     "[| F \<in> A LeadsTo B;  F \<in> B LeadsTo C |] ==> F \<in> A LeadsTo C"
+apply (simp (no_asm_use) add: LeadsTo_def)
+apply (blast intro: leadsTo_Trans)
+done
+
+lemma LeadsTo_Union:
+"[|(!!A. A \<in> S ==> F \<in> A LeadsTo B); F \<in> program|]==>F \<in> Union(S) LeadsTo B"
+apply (simp add: LeadsTo_def)
+apply (subst Int_Union_Union2)
+apply (rule leadsTo_UN, auto)
+done
+
+(*** Derived rules ***)
+
+lemma leadsTo_imp_LeadsTo: "F \<in> A leadsTo B ==> F \<in> A LeadsTo B"
+apply (frule leadsToD2, clarify)
+apply (simp (no_asm_simp) add: LeadsTo_eq)
+apply (blast intro: leadsTo_weaken_L)
+done
+
+(*Useful with cancellation, disjunction*)
+lemma LeadsTo_Un_duplicate: "F \<in> A LeadsTo (A' Un A') ==> F \<in> A LeadsTo A'"
+by (simp add: Un_ac)
+
+lemma LeadsTo_Un_duplicate2:
+     "F \<in> A LeadsTo (A' Un C Un C) ==> F \<in> A LeadsTo (A' Un C)"
+by (simp add: Un_ac)
+
+lemma LeadsTo_UN:
+    "[|(!!i. i \<in> I ==> F \<in> A(i) LeadsTo B); F \<in> program|]
+     ==>F:(\<Union>i \<in> I. A(i)) LeadsTo B"
+apply (simp add: LeadsTo_def)
+apply (simp (no_asm_simp) del: UN_simps add: Int_UN_distrib)
+apply (rule leadsTo_UN, auto)
+done
+
+(*Binary union introduction rule*)
+lemma LeadsTo_Un:
+     "[| F \<in> A LeadsTo C; F \<in> B LeadsTo C |] ==> F \<in> (A Un B) LeadsTo C"
+apply (subst Un_eq_Union)
+apply (rule LeadsTo_Union)
+apply (auto dest: LeadsTo_type [THEN subsetD])
+done
+
+(*Lets us look at the starting state*)
+lemma single_LeadsTo_I: 
+    "[|(!!s. s \<in> A ==> F:{s} LeadsTo B); F \<in> program|]==>F \<in> A LeadsTo B"
+apply (subst UN_singleton [symmetric], rule LeadsTo_UN, auto)
+done
+
+lemma subset_imp_LeadsTo: "[| A <= B; F \<in> program |] ==> F \<in> A LeadsTo B"
+apply (simp (no_asm_simp) add: LeadsTo_def)
+apply (blast intro: subset_imp_leadsTo)
+done
+
+lemma empty_LeadsTo: "F:0 LeadsTo A <-> F \<in> program"
+by (auto dest: LeadsTo_type [THEN subsetD]
+            intro: empty_subsetI [THEN subset_imp_LeadsTo])
+declare empty_LeadsTo [iff]
+
+lemma LeadsTo_state: "F \<in> A LeadsTo state <-> F \<in> program"
+by (auto dest: LeadsTo_type [THEN subsetD] simp add: LeadsTo_eq)
+declare LeadsTo_state [iff]
+
+lemma LeadsTo_weaken_R: "[| F \<in> A LeadsTo A';  A'<=B'|] ==> F \<in> A LeadsTo B'"
+apply (unfold LeadsTo_def)
+apply (auto intro: leadsTo_weaken_R)
+done
+
+lemma LeadsTo_weaken_L: "[| F \<in> A LeadsTo A'; B <= A |] ==> F \<in> B LeadsTo A'"
+apply (unfold LeadsTo_def)
+apply (auto intro: leadsTo_weaken_L)
+done
+
+lemma LeadsTo_weaken: "[| F \<in> A LeadsTo A'; B<=A; A'<=B' |] ==> F \<in> B LeadsTo B'"
+by (blast intro: LeadsTo_weaken_R LeadsTo_weaken_L LeadsTo_Trans)
+
+lemma Always_LeadsTo_weaken: 
+"[| F \<in> Always(C);  F \<in> A LeadsTo A'; C Int B <= A;   C Int A' <= B' |]  
+      ==> F \<in> B LeadsTo B'"
+apply (blast dest: Always_LeadsToI intro: LeadsTo_weaken Always_LeadsToD)
+done
+
+(** Two theorems for "proof lattices" **)
+
+lemma LeadsTo_Un_post: "F \<in> A LeadsTo B ==> F:(A Un B) LeadsTo B"
+by (blast dest: LeadsTo_type [THEN subsetD]
+             intro: LeadsTo_Un subset_imp_LeadsTo)
+
+lemma LeadsTo_Trans_Un: "[| F \<in> A LeadsTo B;  F \<in> B LeadsTo C |]  
+      ==> F \<in> (A Un B) LeadsTo C"
+apply (blast intro: LeadsTo_Un subset_imp_LeadsTo LeadsTo_weaken_L LeadsTo_Trans dest: LeadsTo_type [THEN subsetD])
+done
+
+(** Distributive laws **)
+lemma LeadsTo_Un_distrib: "(F \<in> (A Un B) LeadsTo C)  <-> (F \<in> A LeadsTo C & F \<in> B LeadsTo C)"
+by (blast intro: LeadsTo_Un LeadsTo_weaken_L)
+
+lemma LeadsTo_UN_distrib: "(F \<in> (\<Union>i \<in> I. A(i)) LeadsTo B) <->  (\<forall>i \<in> I. F \<in> A(i) LeadsTo B) & F \<in> program"
+by (blast dest: LeadsTo_type [THEN subsetD]
+             intro: LeadsTo_UN LeadsTo_weaken_L)
+
+lemma LeadsTo_Union_distrib: "(F \<in> Union(S) LeadsTo B)  <->  (\<forall>A \<in> S. F \<in> A LeadsTo B) & F \<in> program"
+by (blast dest: LeadsTo_type [THEN subsetD]
+             intro: LeadsTo_Union LeadsTo_weaken_L)
+
+(** More rules using the premise "Always(I)" **)
+
+lemma EnsuresI: "[| F:(A-B) Co (A Un B);  F \<in> transient (A-B) |] ==> F \<in> A Ensures B"
+apply (simp add: Ensures_def Constrains_eq_constrains)
+apply (blast intro: ensuresI constrains_weaken transient_strengthen dest: constrainsD2)
+done
+
+lemma Always_LeadsTo_Basis: "[| F \<in> Always(I); F \<in> (I Int (A-A')) Co (A Un A');  
+         F \<in> transient (I Int (A-A')) |]    
+  ==> F \<in> A LeadsTo A'"
+apply (rule Always_LeadsToI, assumption)
+apply (blast intro: EnsuresI LeadsTo_Basis Always_ConstrainsD [THEN Constrains_weaken] transient_strengthen)
+done
+
+(*Set difference: maybe combine with leadsTo_weaken_L??
+  This is the most useful form of the "disjunction" rule*)
+lemma LeadsTo_Diff:
+     "[| F \<in> (A-B) LeadsTo C;  F \<in> (A Int B) LeadsTo C |] ==> F \<in> A LeadsTo C"
+by (blast intro: LeadsTo_Un LeadsTo_weaken)
+
+lemma LeadsTo_UN_UN:  
+     "[|(!!i. i \<in> I ==> F \<in> A(i) LeadsTo A'(i)); F \<in> program |]  
+      ==> F \<in> (\<Union>i \<in> I. A(i)) LeadsTo (\<Union>i \<in> I. A'(i))"
+apply (rule LeadsTo_Union, auto) 
+apply (blast intro: LeadsTo_weaken_R)
+done
+
+(*Binary union version*)
+lemma LeadsTo_Un_Un:
+  "[| F \<in> A LeadsTo A'; F \<in> B LeadsTo B' |] ==> F:(A Un B) LeadsTo (A' Un B')"
+by (blast intro: LeadsTo_Un LeadsTo_weaken_R)
+
+(** The cancellation law **)
+
+lemma LeadsTo_cancel2: "[| F \<in> A LeadsTo(A' Un B); F \<in> B LeadsTo B' |] ==> F \<in> A LeadsTo (A' Un B')"
+by (blast intro: LeadsTo_Un_Un subset_imp_LeadsTo LeadsTo_Trans dest: LeadsTo_type [THEN subsetD])
+
+lemma Un_Diff: "A Un (B - A) = A Un B"
+by auto
+
+lemma LeadsTo_cancel_Diff2: "[| F \<in> A LeadsTo (A' Un B); F \<in> (B-A') LeadsTo B' |] ==> F \<in> A LeadsTo (A' Un B')"
+apply (rule LeadsTo_cancel2)
+prefer 2 apply assumption
+apply (simp (no_asm_simp) add: Un_Diff)
+done
+
+lemma LeadsTo_cancel1: "[| F \<in> A LeadsTo (B Un A'); F \<in> B LeadsTo B' |] ==> F \<in> A LeadsTo (B' Un A')"
+apply (simp add: Un_commute)
+apply (blast intro!: LeadsTo_cancel2)
+done
+
+lemma Diff_Un2: "(B - A) Un A = B Un A"
+by auto
+
+lemma LeadsTo_cancel_Diff1: "[| F \<in> A LeadsTo (B Un A'); F \<in> (B-A') LeadsTo B' |] ==> F \<in> A LeadsTo (B' Un A')"
+apply (rule LeadsTo_cancel1)
+prefer 2 apply assumption
+apply (simp (no_asm_simp) add: Diff_Un2)
+done
+
+(** The impossibility law **)
+
+(*The set "A" may be non-empty, but it contains no reachable states*)
+lemma LeadsTo_empty: "F \<in> A LeadsTo 0 ==> F \<in> Always (state -A)"
+apply (simp (no_asm_use) add: LeadsTo_def Always_eq_includes_reachable)
+apply (cut_tac reachable_type)
+apply (auto dest!: leadsTo_empty)
+done
+
+(** PSP \<in> Progress-Safety-Progress **)
+
+(*Special case of PSP \<in> Misra's "stable conjunction"*)
+lemma PSP_Stable: "[| F \<in> A LeadsTo A';  F \<in> Stable(B) |]==> F:(A Int B) LeadsTo (A' Int B)"
+apply (simp add: LeadsTo_def Stable_eq_stable, clarify)
+apply (drule psp_stable, assumption)
+apply (simp add: Int_ac)
+done
+
+lemma PSP_Stable2: "[| F \<in> A LeadsTo A'; F \<in> Stable(B) |] ==> F \<in> (B Int A) LeadsTo (B Int A')"
+apply (simp (no_asm_simp) add: PSP_Stable Int_ac)
+done
+
+lemma PSP: "[| F \<in> A LeadsTo A'; F \<in> B Co B'|]==> F \<in> (A Int B') LeadsTo ((A' Int B) Un (B' - B))"
+apply (simp (no_asm_use) add: LeadsTo_def Constrains_eq_constrains)
+apply (blast dest: psp intro: leadsTo_weaken)
+done
+
+lemma PSP2: "[| F \<in> A LeadsTo A'; F \<in> B Co B' |]==> F:(B' Int A) LeadsTo ((B Int A') Un (B' - B))"
+by (simp (no_asm_simp) add: PSP Int_ac)
+
+lemma PSP_Unless: 
+"[| F \<in> A LeadsTo A'; F \<in> B Unless B'|]==> F:(A Int B) LeadsTo ((A' Int B) Un B')"
+apply (unfold Unless_def)
+apply (drule PSP, assumption)
+apply (blast intro: LeadsTo_Diff LeadsTo_weaken subset_imp_LeadsTo)
+done
+
+(*** Induction rules ***)
+
+(** Meta or object quantifier ????? **)
+lemma LeadsTo_wf_induct: "[| wf(r);      
+         \<forall>m \<in> I. F \<in> (A Int f-``{m}) LeadsTo                      
+                            ((A Int f-``(converse(r) `` {m})) Un B);  
+         field(r)<=I; A<=f-``I; F \<in> program |]  
+      ==> F \<in> A LeadsTo B"
+apply (simp (no_asm_use) add: LeadsTo_def)
+apply auto
+apply (erule_tac I = I and f = f in leadsTo_wf_induct, safe)
+apply (drule_tac [2] x = m in bspec, safe)
+apply (rule_tac [2] A' = "reachable (F) Int (A Int f -`` (converse (r) ``{m}) Un B) " in leadsTo_weaken_R)
+apply (auto simp add: Int_assoc) 
+done
+
+
+lemma LessThan_induct: "[| \<forall>m \<in> nat. F:(A Int f-``{m}) LeadsTo ((A Int f-``m) Un B);  
+      A<=f-``nat; F \<in> program |] ==> F \<in> A LeadsTo B"
+apply (rule_tac A1 = nat and f1 = "%x. x" in wf_measure [THEN LeadsTo_wf_induct])
+apply (simp_all add: nat_measure_field)
+apply (simp add: ltI Image_inverse_lessThan vimage_def [symmetric])
+done
+
+
+(****** 
+ To be ported ??? I am not sure.
+
+  integ_0_le_induct
+  LessThan_bounded_induct
+  GreaterThan_bounded_induct
+
+*****)
+
+(*** Completion \<in> Binary and General Finite versions ***)
+
+lemma Completion: "[| F \<in> A LeadsTo (A' Un C);  F \<in> A' Co (A' Un C);  
+         F \<in> B LeadsTo (B' Un C);  F \<in> B' Co (B' Un C) |]  
+      ==> F \<in> (A Int B) LeadsTo ((A' Int B') Un C)"
+apply (simp (no_asm_use) add: LeadsTo_def Constrains_eq_constrains Int_Un_distrib)
+apply (blast intro: completion leadsTo_weaken)
+done
+
+lemma Finite_completion_aux:
+     "[| I \<in> Fin(X);F \<in> program |]  
+      ==> (\<forall>i \<in> I. F \<in> (A(i)) LeadsTo (A'(i) Un C)) -->   
+          (\<forall>i \<in> I. F \<in> (A'(i)) Co (A'(i) Un C)) -->  
+          F \<in> (\<Inter>i \<in> I. A(i)) LeadsTo ((\<Inter>i \<in> I. A'(i)) Un C)"
+apply (erule Fin_induct)
+apply (auto simp del: INT_simps simp add: Inter_0)
+apply (rule Completion, auto) 
+apply (simp del: INT_simps add: INT_extend_simps)
+apply (blast intro: Constrains_INT)
+done
+
+lemma Finite_completion: 
+     "[| I \<in> Fin(X); !!i. i \<in> I ==> F \<in> A(i) LeadsTo (A'(i) Un C);  
+         !!i. i \<in> I ==> F \<in> A'(i) Co (A'(i) Un C);  
+         F \<in> program |]    
+      ==> F \<in> (\<Inter>i \<in> I. A(i)) LeadsTo ((\<Inter>i \<in> I. A'(i)) Un C)"
+by (blast intro: Finite_completion_aux [THEN mp, THEN mp])
+
+lemma Stable_completion: 
+     "[| F \<in> A LeadsTo A';  F \<in> Stable(A');    
+         F \<in> B LeadsTo B';  F \<in> Stable(B') |]  
+    ==> F \<in> (A Int B) LeadsTo (A' Int B')"
+apply (unfold Stable_def)
+apply (rule_tac C1 = 0 in Completion [THEN LeadsTo_weaken_R])
+    prefer 5
+    apply blast 
+apply auto 
+done
+
+lemma Finite_stable_completion: 
+     "[| I \<in> Fin(X);  
+         (!!i. i \<in> I ==> F \<in> A(i) LeadsTo A'(i));  
+         (!!i. i \<in> I ==>F \<in> Stable(A'(i)));   F \<in> program  |]  
+      ==> F \<in> (\<Inter>i \<in> I. A(i)) LeadsTo (\<Inter>i \<in> I. A'(i))"
+apply (unfold Stable_def)
+apply (rule_tac C1 = 0 in Finite_completion [THEN LeadsTo_weaken_R], simp_all)
+apply (rule_tac [3] subset_refl, auto) 
+done
+
+ML
+{*
+val LeadsTo_eq = thm "LeadsTo_eq";
+val LeadsTo_type = thm "LeadsTo_type";
+val Always_LeadsTo_pre = thm "Always_LeadsTo_pre";
+val Always_LeadsTo_post = thm "Always_LeadsTo_post";
+val Always_LeadsToI = thm "Always_LeadsToI";
+val Always_LeadsToD = thm "Always_LeadsToD";
+val LeadsTo_Basis = thm "LeadsTo_Basis";
+val LeadsTo_Trans = thm "LeadsTo_Trans";
+val LeadsTo_Union = thm "LeadsTo_Union";
+val leadsTo_imp_LeadsTo = thm "leadsTo_imp_LeadsTo";
+val LeadsTo_Un_duplicate = thm "LeadsTo_Un_duplicate";
+val LeadsTo_Un_duplicate2 = thm "LeadsTo_Un_duplicate2";
+val LeadsTo_UN = thm "LeadsTo_UN";
+val LeadsTo_Un = thm "LeadsTo_Un";
+val single_LeadsTo_I = thm "single_LeadsTo_I";
+val subset_imp_LeadsTo = thm "subset_imp_LeadsTo";
+val empty_LeadsTo = thm "empty_LeadsTo";
+val LeadsTo_state = thm "LeadsTo_state";
+val LeadsTo_weaken_R = thm "LeadsTo_weaken_R";
+val LeadsTo_weaken_L = thm "LeadsTo_weaken_L";
+val LeadsTo_weaken = thm "LeadsTo_weaken";
+val Always_LeadsTo_weaken = thm "Always_LeadsTo_weaken";
+val LeadsTo_Un_post = thm "LeadsTo_Un_post";
+val LeadsTo_Trans_Un = thm "LeadsTo_Trans_Un";
+val LeadsTo_Un_distrib = thm "LeadsTo_Un_distrib";
+val LeadsTo_UN_distrib = thm "LeadsTo_UN_distrib";
+val LeadsTo_Union_distrib = thm "LeadsTo_Union_distrib";
+val EnsuresI = thm "EnsuresI";
+val Always_LeadsTo_Basis = thm "Always_LeadsTo_Basis";
+val LeadsTo_Diff = thm "LeadsTo_Diff";
+val LeadsTo_UN_UN = thm "LeadsTo_UN_UN";
+val LeadsTo_Un_Un = thm "LeadsTo_Un_Un";
+val LeadsTo_cancel2 = thm "LeadsTo_cancel2";
+val Un_Diff = thm "Un_Diff";
+val LeadsTo_cancel_Diff2 = thm "LeadsTo_cancel_Diff2";
+val LeadsTo_cancel1 = thm "LeadsTo_cancel1";
+val Diff_Un2 = thm "Diff_Un2";
+val LeadsTo_cancel_Diff1 = thm "LeadsTo_cancel_Diff1";
+val LeadsTo_empty = thm "LeadsTo_empty";
+val PSP_Stable = thm "PSP_Stable";
+val PSP_Stable2 = thm "PSP_Stable2";
+val PSP = thm "PSP";
+val PSP2 = thm "PSP2";
+val PSP_Unless = thm "PSP_Unless";
+val LeadsTo_wf_induct = thm "LeadsTo_wf_induct";
+val LessThan_induct = thm "LessThan_induct";
+val Completion = thm "Completion";
+val Finite_completion = thm "Finite_completion";
+val Stable_completion = thm "Stable_completion";
+val Finite_stable_completion = thm "Finite_stable_completion";
+
+
+(*proves "ensures/leadsTo" properties when the program is specified*)
+fun gen_ensures_tac(cs,ss) sact = 
+    SELECT_GOAL
+      (EVERY [REPEAT (Always_Int_tac 1),
+              etac Always_LeadsTo_Basis 1 
+                  ORELSE   (*subgoal may involve LeadsTo, leadsTo or ensures*)
+                  REPEAT (ares_tac [LeadsTo_Basis, leadsTo_Basis,
+                                    EnsuresI, ensuresI] 1),
+              (*now there are two subgoals: co & transient*)
+              simp_tac (ss addsimps !program_defs_ref) 2,
+              res_inst_tac [("act", sact)] transientI 2,
+                 (*simplify the command's domain*)
+              simp_tac (ss addsimps [domain_def]) 3, 
+              (* proving the domain part *)
+             clarify_tac cs 3, dtac swap 3, force_tac (cs,ss) 4,
+             rtac ReplaceI 3, force_tac (cs,ss) 3, force_tac (cs,ss) 4,
+             asm_full_simp_tac ss 3, rtac conjI 3, simp_tac ss 4,
+             REPEAT (rtac state_update_type 3),
+             gen_constrains_tac (cs,ss) 1,
+             ALLGOALS (clarify_tac cs),
+             ALLGOALS (asm_full_simp_tac (ss addsimps [st_set_def])),
+                        ALLGOALS (clarify_tac cs),
+            ALLGOALS (asm_lr_simp_tac ss)]);
+
+fun ensures_tac sact = gen_ensures_tac (claset(), simpset()) sact;
+*}
+
+
+method_setup ensures_tac = {*
+    fn args => fn ctxt =>
+        Method.goal_args' (Scan.lift Args.name) 
+           (gen_ensures_tac (local_clasimpset_of ctxt))
+           args ctxt *}
+    "for proving progress properties"
+
 
 end
