src/ZF/UNITY/GenPrefix.thy
@@ -1,9 +1,7 @@
-(*  Title:      ZF/UNITY/GenPrefix.thy
-    ID:         $Id$
+(*  ID:         $Id$
     Author:     Sidi O Ehmety, Cambridge University Computer Laboratory
     Copyright   2001  University of Cambridge
 
-Charpentier's Generalized Prefix Relation
    <xs,ys>:gen_prefix(r)
      if ys = xs' @ zs where length(xs) = length(xs')
      and corresponding elements of xs, xs' are pairwise related by r
@@ -11,10 +9,15 @@ Charpentier's Generalized Prefix Relation
 Based on Lex/Prefix
 *)
 
-GenPrefix = Main + 
+header{*Charpentier's Generalized Prefix Relation*}
+
+theory GenPrefix
+imports Main 
+
+begin
 
 constdefs (*really belongs in ZF/Trancl*)
-  part_order :: [i, i] => o
+  part_order :: "[i, i] => o"
   "part_order(A, r) == refl(A,r) & trans[A](r) & antisym(r)"
 
 consts
@@ -25,31 +28,651 @@ inductive
   
   domains "gen_prefix(A, r)" <= "list(A)*list(A)"
   
-  intrs
-    Nil     "<[],[]>:gen_prefix(A, r)"
+  intros
+    Nil:     "<[],[]>:gen_prefix(A, r)"
 
-    prepend "[| <xs,ys>:gen_prefix(A, r);  <x,y>:r; x:A; y:A |]
+    prepend: "[| <xs,ys>:gen_prefix(A, r);  <x,y>:r; x:A; y:A |]
 	      ==> <Cons(x,xs), Cons(y,ys)>: gen_prefix(A, r)"
 
-    append  "[| <xs,ys>:gen_prefix(A, r); zs:list(A) |]
-	     ==> <xs, ys@zs>:gen_prefix(A, r)"
-    type_intrs "list.intrs@[app_type]"
+    append:  "[| <xs,ys>:gen_prefix(A, r); zs:list(A) |]
+	      ==> <xs, ys@zs>:gen_prefix(A, r)"
+    type_intros app_type list.Nil list.Cons
 
 constdefs
-   prefix :: i=>i
+   prefix :: "i=>i"
   "prefix(A) == gen_prefix(A, id(A))"
 
-   strict_prefix :: i=>i  
+   strict_prefix :: "i=>i"
   "strict_prefix(A) == prefix(A) - id(list(A))"
 
 syntax
   (* less or equal and greater or equal over prefixes *)
-  pfixLe :: [i, i] => o               (infixl "pfixLe" 50)
-  pfixGe :: [i, i] => o               (infixl "pfixGe" 50)
+  pfixLe :: "[i, i] => o"               (infixl "pfixLe" 50)
+  pfixGe :: "[i, i] => o"               (infixl "pfixGe" 50)
 
 translations
    "xs pfixLe ys" == "<xs, ys>:gen_prefix(nat, Le)"
    "xs pfixGe ys" == "<xs, ys>:gen_prefix(nat, Ge)"
   
+
+lemma reflD: 
+ "[| refl(A, r); x \<in> A |] ==> <x,x>:r"
+apply (unfold refl_def, auto)
+done
+
+(*** preliminary lemmas ***)
+
+lemma Nil_gen_prefix: "xs \<in> list(A) ==> <[], xs> \<in> gen_prefix(A, r)"
+by (drule gen_prefix.append [OF gen_prefix.Nil], simp)
+declare Nil_gen_prefix [simp]
+
+
+lemma gen_prefix_length_le: "<xs,ys> \<in> gen_prefix(A, r) ==> length(xs) \<le> length(ys)"
+apply (erule gen_prefix.induct)
+apply (subgoal_tac [3] "ys \<in> list (A) ")
+apply (auto dest: gen_prefix.dom_subset [THEN subsetD]
+            intro: le_trans simp add: length_app)
+done
+
+
+lemma Cons_gen_prefix_aux:
+  "[| <xs', ys'> \<in> gen_prefix(A, r) |]  
+   ==> (\<forall>x xs. x \<in> A --> xs'= Cons(x,xs) -->  
+       (\<exists>y ys. y \<in> A & ys' = Cons(y,ys) & 
+       <x,y>:r & <xs, ys> \<in> gen_prefix(A, r)))"
+apply (erule gen_prefix.induct)
+prefer 3 apply (force intro: gen_prefix.append, auto) 
+done
+
+lemma Cons_gen_prefixE:
+  "[| <Cons(x,xs), zs> \<in> gen_prefix(A, r);  
+    !!y ys. [|zs = Cons(y, ys); y \<in> A; x \<in> A; <x,y>:r;  
+      <xs,ys> \<in> gen_prefix(A, r) |] ==> P |] ==> P"
+apply (frule gen_prefix.dom_subset [THEN subsetD], auto) 
+apply (blast dest: Cons_gen_prefix_aux) 
+done
+declare Cons_gen_prefixE [elim!]
+
+lemma Cons_gen_prefix_Cons: 
+"(<Cons(x,xs),Cons(y,ys)> \<in> gen_prefix(A, r))  
+  <-> (x \<in> A & y \<in> A & <x,y>:r & <xs,ys> \<in> gen_prefix(A, r))"
+apply (auto intro: gen_prefix.prepend)
+done
+declare Cons_gen_prefix_Cons [iff]
+
+(** Monotonicity of gen_prefix **)
+
+lemma gen_prefix_mono2: "r<=s ==> gen_prefix(A, r) <= gen_prefix(A, s)"
+apply clarify
+apply (frule gen_prefix.dom_subset [THEN subsetD], clarify)
+apply (erule rev_mp)
+apply (erule gen_prefix.induct)
+apply (auto intro: gen_prefix.append)
+done
+
+lemma gen_prefix_mono1: "A<=B ==>gen_prefix(A, r) <= gen_prefix(B, r)"
+apply clarify
+apply (frule gen_prefix.dom_subset [THEN subsetD], clarify)
+apply (erule rev_mp)
+apply (erule_tac P = "y \<in> list (A) " in rev_mp)
+apply (erule_tac P = "xa \<in> list (A) " in rev_mp)
+apply (erule gen_prefix.induct)
+apply (simp (no_asm_simp))
+apply clarify
+apply (erule ConsE)+
+apply (auto dest: gen_prefix.dom_subset [THEN subsetD]
+            intro: gen_prefix.append list_mono [THEN subsetD])
+done
+
+lemma gen_prefix_mono: "[| A <= B; r <= s |] ==> gen_prefix(A, r) <= gen_prefix(B, s)"
+apply (rule subset_trans)
+apply (rule gen_prefix_mono1)
+apply (rule_tac [2] gen_prefix_mono2, auto)
+done
+
+(*** gen_prefix order ***)
+
+(* reflexivity *)
+lemma refl_gen_prefix: "refl(A, r) ==> refl(list(A), gen_prefix(A, r))"
+apply (unfold refl_def, auto)
+apply (induct_tac "x", auto)
+done
+declare refl_gen_prefix [THEN reflD, simp]
+
+(* Transitivity *)
+(* A lemma for proving gen_prefix_trans_comp *)
+
+lemma append_gen_prefix [rule_format (no_asm)]: "xs \<in> list(A) ==>  
+   \<forall>zs. <xs @ ys, zs> \<in> gen_prefix(A, r) --> <xs, zs>: gen_prefix(A, r)"
+apply (erule list.induct)
+apply (auto dest: gen_prefix.dom_subset [THEN subsetD])
+done
+
+(* Lemma proving transitivity and more*)
+
+lemma gen_prefix_trans_comp [rule_format (no_asm)]:
+     "<x, y>: gen_prefix(A, r) ==>  
+   (\<forall>z \<in> list(A). <y,z> \<in> gen_prefix(A, s)--><x, z> \<in> gen_prefix(A, s O r))"
+apply (erule gen_prefix.induct)
+apply (auto elim: ConsE simp add: Nil_gen_prefix)
+apply (subgoal_tac "ys \<in> list (A) ")
+prefer 2 apply (blast dest: gen_prefix.dom_subset [THEN subsetD])
+apply (drule_tac xs = ys and r = s in append_gen_prefix, auto)
+done
+
+lemma trans_comp_subset: "trans(r) ==> r O r <= r"
+by (auto dest: transD)
+
+lemma trans_gen_prefix: "trans(r) ==> trans(gen_prefix(A,r))"
+apply (simp (no_asm) add: trans_def)
+apply clarify
+apply (rule trans_comp_subset [THEN gen_prefix_mono2, THEN subsetD], assumption)
+apply (rule gen_prefix_trans_comp)
+apply (auto dest: gen_prefix.dom_subset [THEN subsetD])
+done
+
+lemma trans_on_gen_prefix: 
+ "trans(r) ==> trans[list(A)](gen_prefix(A, r))"
+apply (drule_tac A = A in trans_gen_prefix)
+apply (unfold trans_def trans_on_def, blast)
+done
+
+lemma prefix_gen_prefix_trans:
+    "[| <x,y> \<in> prefix(A); <y, z> \<in> gen_prefix(A, r); r<=A*A |]  
+      ==>  <x, z> \<in> gen_prefix(A, r)"
+apply (unfold prefix_def)
+apply (rule_tac P = "%r. <x,z> \<in> gen_prefix (A, r) " in right_comp_id [THEN subst])
+apply (blast dest: gen_prefix_trans_comp gen_prefix.dom_subset [THEN subsetD])+
+done
+
+
+lemma gen_prefix_prefix_trans: 
+"[| <x,y> \<in> gen_prefix(A,r); <y, z> \<in> prefix(A); r<=A*A |]  
+  ==>  <x, z> \<in> gen_prefix(A, r)"
+apply (unfold prefix_def)
+apply (rule_tac P = "%r. <x,z> \<in> gen_prefix (A, r) " in left_comp_id [THEN subst])
+apply (blast dest: gen_prefix_trans_comp gen_prefix.dom_subset [THEN subsetD])+
+done
+
+(** Antisymmetry **)
+
+lemma nat_le_lemma [rule_format]: "n \<in> nat ==> \<forall>b \<in> nat. n #+ b \<le> n --> b = 0"
+by (induct_tac "n", auto)
+
+lemma antisym_gen_prefix: "antisym(r) ==> antisym(gen_prefix(A, r))"
+apply (simp (no_asm) add: antisym_def)
+apply (rule impI [THEN allI, THEN allI])
+apply (erule gen_prefix.induct, blast) 
+apply (simp add: antisym_def, blast)
+txt{*append case is hardest*}
+apply clarify
+apply (subgoal_tac "length (zs) = 0")
+apply (subgoal_tac "ys \<in> list (A) ")
+prefer 2 apply (blast dest: gen_prefix.dom_subset [THEN subsetD])
+apply (drule_tac psi = "<ys @ zs, xs> \<in> gen_prefix (A,r) " in asm_rl)
+apply simp
+apply (subgoal_tac "length (ys @ zs) = length (ys) #+ length (zs) &ys \<in> list (A) &xs \<in> list (A) ")
+prefer 2 apply (blast intro: length_app dest: gen_prefix.dom_subset [THEN subsetD])
+apply (drule gen_prefix_length_le)+
+apply clarify
+apply simp
+apply (drule_tac j = "length (xs) " in le_trans)
+apply blast
+apply (auto intro: nat_le_lemma)
+done
+
+(*** recursion equations ***)
+
+lemma gen_prefix_Nil: "xs \<in> list(A) ==> <xs, []> \<in> gen_prefix(A,r) <-> (xs = [])"
+by (induct_tac "xs", auto)
+declare gen_prefix_Nil [simp]
+
+lemma same_gen_prefix_gen_prefix: 
+ "[| refl(A, r);  xs \<in> list(A) |] ==>  
+    <xs@ys, xs@zs>: gen_prefix(A, r) <-> <ys,zs> \<in> gen_prefix(A, r)"
+apply (unfold refl_def)
+apply (induct_tac "xs")
+apply (simp_all (no_asm_simp))
+done
+declare same_gen_prefix_gen_prefix [simp]
+
+lemma gen_prefix_Cons: "[| xs \<in> list(A); ys \<in> list(A); y \<in> A |] ==>  
+    <xs, Cons(y,ys)> \<in> gen_prefix(A,r)  <->  
+      (xs=[] | (\<exists>z zs. xs=Cons(z,zs) & z \<in> A & <z,y>:r & <zs,ys> \<in> gen_prefix(A,r)))"
+apply (induct_tac "xs", auto)
+done
+
+lemma gen_prefix_take_append: "[| refl(A,r);  <xs,ys> \<in> gen_prefix(A, r); zs \<in> list(A) |]  
+      ==>  <xs@zs, take(length(xs), ys) @ zs> \<in> gen_prefix(A, r)"
+apply (erule gen_prefix.induct)
+apply (simp (no_asm_simp))
+apply (frule_tac [!] gen_prefix.dom_subset [THEN subsetD], auto)
+apply (frule gen_prefix_length_le)
+apply (subgoal_tac "take (length (xs), ys) \<in> list (A) ")
+apply (simp_all (no_asm_simp) add: diff_is_0_iff [THEN iffD2] take_type)
+done
+
+lemma gen_prefix_append_both: "[| refl(A, r);  <xs,ys> \<in> gen_prefix(A,r);    
+         length(xs) = length(ys); zs \<in> list(A) |]  
+      ==>  <xs@zs, ys @ zs> \<in> gen_prefix(A, r)"
+apply (drule_tac zs = zs in gen_prefix_take_append, assumption+)
+apply (subgoal_tac "take (length (xs), ys) =ys")
+apply (auto intro!: take_all dest: gen_prefix.dom_subset [THEN subsetD])
+done
+
+(*NOT suitable for rewriting since [y] has the form y#ys*)
+lemma append_cons_conv: "xs \<in> list(A) ==> xs @ Cons(y, ys) = (xs @ [y]) @ ys"
+by (auto simp add: app_assoc)
+
+lemma append_one_gen_prefix_lemma [rule_format]:
+     "[| <xs,ys> \<in> gen_prefix(A, r);  refl(A, r) |]  
+      ==> length(xs) < length(ys) -->  
+          <xs @ [nth(length(xs), ys)], ys> \<in> gen_prefix(A, r)"
+apply (erule gen_prefix.induct, blast)
+apply (frule gen_prefix.dom_subset [THEN subsetD], clarify)
+apply (simp_all add: length_type)
+(* Append case is hardest *)
+apply (frule gen_prefix_length_le [THEN le_iff [THEN iffD1]])
+apply (frule gen_prefix.dom_subset [THEN subsetD], clarify)
+apply (subgoal_tac "length (xs) :nat&length (ys) :nat &length (zs) :nat")
+prefer 2 apply (blast intro: length_type, clarify)
+apply (simp_all add: nth_append length_type length_app)
+apply (rule conjI)
+apply (blast intro: gen_prefix.append)
+apply (erule_tac V = "length (xs) < length (ys) -->?u" in thin_rl)
+apply (erule_tac a = zs in list.cases, auto)
+apply (rule_tac P1 = "%x. <?u (x), ?v>:?w" in nat_diff_split [THEN iffD2])
+apply auto
+apply (simplesubst append_cons_conv)
+apply (rule_tac [2] gen_prefix.append)
+apply (auto elim: ConsE simp add: gen_prefix_append_both)
+done 
+
+lemma append_one_gen_prefix: "[| <xs,ys>: gen_prefix(A, r);  length(xs) < length(ys);  refl(A, r) |]  
+      ==> <xs @ [nth(length(xs), ys)], ys> \<in> gen_prefix(A, r)"
+apply (blast intro: append_one_gen_prefix_lemma)
+done
+
+
+(** Proving the equivalence with Charpentier's definition **)
+
+lemma gen_prefix_imp_nth_lemma [rule_format]: "xs \<in> list(A) ==>   
+  \<forall>ys \<in> list(A). \<forall>i \<in> nat. i < length(xs)  
+          --> <xs, ys>: gen_prefix(A, r) --> <nth(i, xs), nth(i, ys)>:r"
+apply (induct_tac "xs", simp, clarify) 
+apply simp 
+apply (erule natE, auto) 
+done
+
+lemma gen_prefix_imp_nth: "[| <xs,ys> \<in> gen_prefix(A,r); i < length(xs)|]  
+      ==> <nth(i, xs), nth(i, ys)>:r"
+apply (cut_tac A = A in gen_prefix.dom_subset)
+apply (rule gen_prefix_imp_nth_lemma)
+apply (auto simp add: lt_nat_in_nat)
+done
+
+lemma nth_imp_gen_prefix [rule_format]: "xs \<in> list(A) ==>  
+  \<forall>ys \<in> list(A). length(xs) \<le> length(ys)   
+      --> (\<forall>i. i < length(xs) --> <nth(i, xs), nth(i,ys)>:r)   
+      --> <xs, ys> \<in> gen_prefix(A, r)"
+apply (induct_tac "xs")
+apply (simp_all (no_asm_simp))
+apply clarify
+apply (erule_tac a = ys in list.cases, simp)
+apply (force intro!: nat_0_le simp add: lt_nat_in_nat)
+done
+
+lemma gen_prefix_iff_nth: "(<xs,ys> \<in> gen_prefix(A,r)) <->  
+      (xs \<in> list(A) & ys \<in> list(A) & length(xs) \<le> length(ys) &  
+      (\<forall>i. i < length(xs) --> <nth(i,xs), nth(i, ys)>: r))"
+apply (rule iffI)
+apply (frule gen_prefix.dom_subset [THEN subsetD])
+apply (frule gen_prefix_length_le, auto) 
+apply (rule_tac [2] nth_imp_gen_prefix)
+apply (drule gen_prefix_imp_nth)
+apply (auto simp add: lt_nat_in_nat)
+done
+
+(** prefix is a partial order: **)
+
+lemma refl_prefix: "refl(list(A), prefix(A))"
+apply (unfold prefix_def)
+apply (rule refl_gen_prefix)
+apply (auto simp add: refl_def)
+done
+declare refl_prefix [THEN reflD, simp]
+
+lemma trans_prefix: "trans(prefix(A))"
+apply (unfold prefix_def)
+apply (rule trans_gen_prefix)
+apply (auto simp add: trans_def)
+done
+
+lemmas prefix_trans = trans_prefix [THEN transD, standard]
+
+lemma trans_on_prefix: "trans[list(A)](prefix(A))"
+apply (unfold prefix_def)
+apply (rule trans_on_gen_prefix)
+apply (auto simp add: trans_def)
+done
+
+lemmas prefix_trans_on = trans_on_prefix [THEN trans_onD, standard]
+
+(* Monotonicity of "set" operator WRT prefix *)
+
+lemma set_of_list_prefix_mono: 
+"<xs,ys> \<in> prefix(A) ==> set_of_list(xs) <= set_of_list(ys)"
+
+apply (unfold prefix_def)
+apply (erule gen_prefix.induct)
+apply (subgoal_tac [3] "xs \<in> list (A) &ys \<in> list (A) ")
+prefer 4 apply (blast dest: gen_prefix.dom_subset [THEN subsetD])
+apply (auto simp add: set_of_list_append)
+done
+
+(** recursion equations **)
+
+lemma Nil_prefix: "xs \<in> list(A) ==> <[],xs> \<in> prefix(A)"
+
+apply (unfold prefix_def)
+apply (simp (no_asm_simp) add: Nil_gen_prefix)
+done
+declare Nil_prefix [simp]
+
+
+lemma prefix_Nil: "<xs, []> \<in> prefix(A) <-> (xs = [])"
+
+apply (unfold prefix_def, auto)
+apply (frule gen_prefix.dom_subset [THEN subsetD])
+apply (drule_tac psi = "<xs, []> \<in> gen_prefix (A, id (A))" in asm_rl)
+apply (simp add: gen_prefix_Nil)
+done
+declare prefix_Nil [iff]
+
+lemma Cons_prefix_Cons: 
+"<Cons(x,xs), Cons(y,ys)> \<in> prefix(A) <-> (x=y & <xs,ys> \<in> prefix(A) & y \<in> A)"
+apply (unfold prefix_def, auto)
+done
+declare Cons_prefix_Cons [iff]
+
+lemma same_prefix_prefix: 
+"xs \<in> list(A)==> <xs@ys,xs@zs> \<in> prefix(A) <-> (<ys,zs> \<in> prefix(A))"
+apply (unfold prefix_def)
+apply (subgoal_tac "refl (A,id (A))")
+apply (simp (no_asm_simp))
+apply (auto simp add: refl_def)
+done
+declare same_prefix_prefix [simp]
+
+lemma same_prefix_prefix_Nil: "xs \<in> list(A) ==> <xs@ys,xs> \<in> prefix(A) <-> (<ys,[]> \<in> prefix(A))"
+apply (rule_tac P = "%x. <?u, x>:?v <-> ?w (x) " in app_right_Nil [THEN subst])
+apply (rule_tac [2] same_prefix_prefix, auto)
+done
+declare same_prefix_prefix_Nil [simp]
+
+lemma prefix_appendI: 
+"[| <xs,ys> \<in> prefix(A); zs \<in> list(A) |] ==> <xs,ys@zs> \<in> prefix(A)"
+apply (unfold prefix_def)
+apply (erule gen_prefix.append, assumption)
+done
+declare prefix_appendI [simp]
+
+lemma prefix_Cons: 
+"[| xs \<in> list(A); ys \<in> list(A); y \<in> A |] ==>  
+  <xs,Cons(y,ys)> \<in> prefix(A) <->  
+  (xs=[] | (\<exists>zs. xs=Cons(y,zs) & <zs,ys> \<in> prefix(A)))"
+apply (unfold prefix_def)
+apply (auto simp add: gen_prefix_Cons)
+done
+
+lemma append_one_prefix: 
+  "[| <xs,ys> \<in> prefix(A); length(xs) < length(ys) |]  
+  ==> <xs @ [nth(length(xs),ys)], ys> \<in> prefix(A)"
+apply (unfold prefix_def)
+apply (subgoal_tac "refl (A, id (A))")
+apply (simp (no_asm_simp) add: append_one_gen_prefix)
+apply (auto simp add: refl_def)
+done
+
+lemma prefix_length_le: 
+"<xs,ys> \<in> prefix(A) ==> length(xs) \<le> length(ys)"
+apply (unfold prefix_def)
+apply (blast dest: gen_prefix_length_le)
+done
+
+lemma prefix_type: "prefix(A)<=list(A)*list(A)"
+apply (unfold prefix_def)
+apply (blast intro!: gen_prefix.dom_subset)
+done
+
+lemma strict_prefix_type: 
+"strict_prefix(A) <= list(A)*list(A)"
+apply (unfold strict_prefix_def)
+apply (blast intro!: prefix_type [THEN subsetD])
+done
+
+lemma strict_prefix_length_lt_aux: 
+     "<xs,ys> \<in> prefix(A) ==> xs\<noteq>ys --> length(xs) < length(ys)"
+apply (unfold prefix_def)
+apply (erule gen_prefix.induct, clarify)
+apply (subgoal_tac [!] "ys \<in> list(A) & xs \<in> list(A)")
+apply (auto dest: gen_prefix.dom_subset [THEN subsetD]
+            simp add: length_type)
+apply (subgoal_tac "length (zs) =0")
+apply (drule_tac [2] not_lt_imp_le)
+apply (rule_tac [5] j = "length (ys) " in lt_trans2)
+apply auto
+done
+
+lemma strict_prefix_length_lt: 
+     "<xs,ys>:strict_prefix(A) ==> length(xs) < length(ys)"
+apply (unfold strict_prefix_def)
+apply (rule strict_prefix_length_lt_aux [THEN mp])
+apply (auto dest: prefix_type [THEN subsetD])
+done
+
+(*Equivalence to the definition used in Lex/Prefix.thy*)
+lemma prefix_iff: 
+    "<xs,zs> \<in> prefix(A) <-> (\<exists>ys \<in> list(A). zs = xs@ys) & xs \<in> list(A)"
+apply (unfold prefix_def)
+apply (auto simp add: gen_prefix_iff_nth lt_nat_in_nat nth_append nth_type app_type length_app)
+apply (subgoal_tac "drop (length (xs), zs) \<in> list (A) ")
+apply (rule_tac x = "drop (length (xs), zs) " in bexI)
+apply safe
+ prefer 2 apply (simp add: length_type drop_type)
+apply (rule nth_equalityI)
+apply (simp_all (no_asm_simp) add: nth_append app_type drop_type length_app length_drop)
+apply (rule nat_diff_split [THEN iffD2], simp_all, clarify)
+apply (drule_tac i = "length (zs) " in leI)
+apply (force simp add: le_subset_iff, safe)
+apply (subgoal_tac "length (xs) #+ (i #- length (xs)) = i")
+apply (subst nth_drop)
+apply (simp_all (no_asm_simp) add: leI split add: nat_diff_split)
+done
+
+lemma prefix_snoc: 
+"[|xs \<in> list(A); ys \<in> list(A); y \<in> A |] ==>  
+   <xs, ys@[y]> \<in> prefix(A) <-> (xs = ys@[y] | <xs,ys> \<in> prefix(A))"
+apply (simp (no_asm) add: prefix_iff)
+apply (rule iffI, clarify)
+apply (erule_tac xs = ysa in rev_list_elim, simp)
+apply (simp add: app_type app_assoc [symmetric])
+apply (auto simp add: app_assoc app_type)
+done
+declare prefix_snoc [simp]
+
+lemma prefix_append_iff [rule_format]: "zs \<in> list(A) ==> \<forall>xs \<in> list(A). \<forall>ys \<in> list(A).  
+   (<xs, ys@zs> \<in> prefix(A)) <->  
+  (<xs,ys> \<in> prefix(A) | (\<exists>us. xs = ys@us & <us,zs> \<in> prefix(A)))"
+apply (erule list_append_induct, force, clarify) 
+apply (rule iffI) 
+apply (simp add: add: app_assoc [symmetric])
+apply (erule disjE)  
+apply (rule disjI2) 
+apply (rule_tac x = "y @ [x]" in exI) 
+apply (simp add: add: app_assoc [symmetric], force+)
+done
+
+
+(*Although the prefix ordering is not linear, the prefixes of a list
+  are linearly ordered.*)
+lemma common_prefix_linear_lemma [rule_format]: "[| zs \<in> list(A); xs \<in> list(A); ys \<in> list(A) |]  
+   ==> <xs, zs> \<in> prefix(A) --> <ys,zs> \<in> prefix(A)  
+  --><xs,ys> \<in> prefix(A) | <ys,xs> \<in> prefix(A)"
+apply (erule list_append_induct, auto)
+done
+
+lemma common_prefix_linear: "[|<xs, zs> \<in> prefix(A); <ys,zs> \<in> prefix(A) |]    
+      ==> <xs,ys> \<in> prefix(A) | <ys,xs> \<in> prefix(A)"
+apply (cut_tac prefix_type)
+apply (blast del: disjCI intro: common_prefix_linear_lemma)
+done
+
+
+(*** pfixLe, pfixGe \<in> properties inherited from the translations ***)
+
+
+
+(** pfixLe **)
+
+lemma refl_Le: "refl(nat,Le)"
+
+apply (unfold refl_def, auto)
+done
+declare refl_Le [simp]
+
+lemma antisym_Le: "antisym(Le)"
+apply (unfold antisym_def)
+apply (auto intro: le_anti_sym)
+done
+declare antisym_Le [simp]
+
+lemma trans_on_Le: "trans[nat](Le)"
+apply (unfold trans_on_def, auto)
+apply (blast intro: le_trans)
+done
+declare trans_on_Le [simp]
+
+lemma trans_Le: "trans(Le)"
+apply (unfold trans_def, auto)
+apply (blast intro: le_trans)
+done
+declare trans_Le [simp]
+
+lemma part_order_Le: "part_order(nat,Le)"
+by (unfold part_order_def, auto)
+declare part_order_Le [simp]
+
+lemma pfixLe_refl: "x \<in> list(nat) ==> x pfixLe x"
+by (blast intro: refl_gen_prefix [THEN reflD] refl_Le)
+declare pfixLe_refl [simp]
+
+lemma pfixLe_trans: "[| x pfixLe y; y pfixLe z |] ==> x pfixLe z"
+by (blast intro: trans_gen_prefix [THEN transD] trans_Le)
+
+lemma pfixLe_antisym: "[| x pfixLe y; y pfixLe x |] ==> x = y"
+by (blast intro: antisym_gen_prefix [THEN antisymE] antisym_Le)
+
+
+lemma prefix_imp_pfixLe: 
+"<xs,ys>:prefix(nat)==> xs pfixLe ys"
+
+apply (unfold prefix_def)
+apply (rule gen_prefix_mono [THEN subsetD], auto)
+done
+
+lemma refl_Ge: "refl(nat, Ge)"
+by (unfold refl_def Ge_def, auto)
+declare refl_Ge [iff]
+
+lemma antisym_Ge: "antisym(Ge)"
+apply (unfold antisym_def Ge_def)
+apply (auto intro: le_anti_sym)
+done
+declare antisym_Ge [iff]
+
+lemma trans_Ge: "trans(Ge)"
+apply (unfold trans_def Ge_def)
+apply (auto intro: le_trans)
+done
+declare trans_Ge [iff]
+
+lemma pfixGe_refl: "x \<in> list(nat) ==> x pfixGe x"
+by (blast intro: refl_gen_prefix [THEN reflD])
+declare pfixGe_refl [simp]
+
+lemma pfixGe_trans: "[| x pfixGe y; y pfixGe z |] ==> x pfixGe z"
+by (blast intro: trans_gen_prefix [THEN transD])
+
+lemma pfixGe_antisym: "[| x pfixGe y; y pfixGe x |] ==> x = y"
+by (blast intro: antisym_gen_prefix [THEN antisymE])
+
+lemma prefix_imp_pfixGe: 
+  "<xs,ys>:prefix(nat) ==> xs pfixGe ys"
+apply (unfold prefix_def Ge_def)
+apply (rule gen_prefix_mono [THEN subsetD], auto)
+done
+(* Added by Sidi \<in> prefix and take *)
+
+lemma prefix_imp_take: 
+"<xs, ys> \<in> prefix(A) ==> xs = take(length(xs), ys)"
+
+apply (unfold prefix_def)
+apply (erule gen_prefix.induct)
+apply (subgoal_tac [3] "length (xs) :nat")
+apply (auto dest: gen_prefix.dom_subset [THEN subsetD] simp add: length_type)
+apply (frule gen_prefix.dom_subset [THEN subsetD])
+apply (frule gen_prefix_length_le)
+apply (auto simp add: take_append)
+apply (subgoal_tac "length (xs) #- length (ys) =0")
+apply (simp_all (no_asm_simp) add: diff_is_0_iff)
+done
+
+lemma prefix_length_equal: "[|<xs,ys> \<in> prefix(A); length(xs)=length(ys)|] ==> xs = ys"
+apply (cut_tac A = A in prefix_type)
+apply (drule subsetD, auto)
+apply (drule prefix_imp_take)
+apply (erule trans, simp)
+done
+
+lemma prefix_length_le_equal: "[|<xs,ys> \<in> prefix(A); length(ys) \<le> length(xs)|] ==> xs = ys"
+by (blast intro: prefix_length_equal le_anti_sym prefix_length_le)
+
+lemma take_prefix [rule_format]: "xs \<in> list(A) ==> \<forall>n \<in> nat. <take(n, xs), xs> \<in> prefix(A)"
+apply (unfold prefix_def)
+apply (erule list.induct, simp, clarify)
+apply (erule natE, auto)
+done
+
+lemma prefix_take_iff: "<xs,ys> \<in> prefix(A) <-> (xs=take(length(xs), ys) & xs \<in> list(A) & ys \<in> list(A))"
+apply (rule iffI)
+apply (frule prefix_type [THEN subsetD])
+apply (blast intro: prefix_imp_take, clarify)
+apply (erule ssubst)
+apply (blast intro: take_prefix length_type)
+done
+
+lemma prefix_imp_nth: "[| <xs,ys> \<in> prefix(A); i < length(xs)|] ==> nth(i,xs) = nth(i,ys)"
+by (auto dest!: gen_prefix_imp_nth simp add: prefix_def)
+
+lemma nth_imp_prefix: 
+     "[|xs \<in> list(A); ys \<in> list(A); length(xs) \<le> length(ys);   
+        !!i. i < length(xs) ==> nth(i, xs) = nth(i,ys)|]   
+      ==> <xs,ys> \<in> prefix(A)"
+apply (auto simp add: prefix_def nth_imp_gen_prefix)
+apply (auto intro!: nth_imp_gen_prefix simp add: prefix_def)
+apply (blast intro: nth_type lt_trans2)
+done
+
+
+lemma length_le_prefix_imp_prefix: "[|length(xs) \<le> length(ys);  
+        <xs,zs> \<in> prefix(A); <ys,zs> \<in> prefix(A)|] ==> <xs,ys> \<in> prefix(A)"
+apply (cut_tac A = A in prefix_type)
+apply (rule nth_imp_prefix, blast, blast)
+ apply assumption
+apply (rule_tac b = "nth (i,zs)" in trans)
+ apply (blast intro: prefix_imp_nth)
+apply (blast intro: sym prefix_imp_nth prefix_length_le lt_trans2)
+done
 
 end
