src/ZF/UNITY/WFair.thy
@@ -2,15 +2,18 @@
     ID:         $Id$
     Author:     Sidi Ehmety, Computer Laboratory
     Copyright   1998  University of Cambridge
-
-Weak Fairness versions of transient, ensures, leadsTo.
-
-From Misra, "A Logic for Concurrent Programming", 1994
-
-Theory ported from HOL.
 *)
 
-WFair = UNITY + Main_ZFC + 
+header{*Progress under Weak Fairness*}
+
+theory WFair
+imports UNITY Main_ZFC
+begin
+
+text{*This theory defines the operators transient, ensures and leadsTo,
+assuming weak fairness. From Misra, "A Logic for Concurrent Programming",
+1994.*}
+
 constdefs
   
   (* This definition specifies weak fairness.  The rest of the theory
@@ -19,7 +22,7 @@ constdefs
   "transient(A) =={F:program. (EX act: Acts(F). A<=domain(act) &
 			       act``A <= state-A) & st_set(A)}"
 
-  ensures :: "[i,i] => i"       (infixl 60)
+  ensures :: "[i,i] => i"       (infixl "ensures" 60)
   "A ensures B == ((A-B) co (A Un B)) Int transient(A-B)"
   
 consts
@@ -30,19 +33,19 @@ consts
 inductive 
   domains
      "leads(D, F)" <= "Pow(D)*Pow(D)"
-  intrs 
-    Basis  "[| F:A ensures B;  A:Pow(D); B:Pow(D) |] ==> <A,B>:leads(D, F)"
-    Trans  "[| <A,B> : leads(D, F); <B,C> : leads(D, F) |] ==>  <A,C>:leads(D, F)"
-    Union   "[| S:Pow({A:S. <A, B>:leads(D, F)}); B:Pow(D); S:Pow(Pow(D)) |] ==> 
+  intros 
+    Basis:  "[| F:A ensures B;  A:Pow(D); B:Pow(D) |] ==> <A,B>:leads(D, F)"
+    Trans:  "[| <A,B> : leads(D, F); <B,C> : leads(D, F) |] ==>  <A,C>:leads(D, F)"
+    Union:   "[| S:Pow({A:S. <A, B>:leads(D, F)}); B:Pow(D); S:Pow(Pow(D)) |] ==> 
 	      <Union(S),B>:leads(D, F)"
 
   monos        Pow_mono
-  type_intrs  "[Union_Pow_iff RS iffD2, UnionI, PowI]"
+  type_intros  Union_Pow_iff [THEN iffD2] UnionI PowI
  
 constdefs
 
   (* The Visible version of the LEADS-TO relation*)
-  leadsTo :: "[i, i] => i"       (infixl 60)
+  leadsTo :: "[i, i] => i"       (infixl "leadsTo" 60)
   "A leadsTo B == {F:program. <A,B>:leads(state, F)}"
   
   (* wlt(F, B) is the largest set that leads to B*)
@@ -50,6 +53,748 @@ constdefs
     "wlt(F, B) == Union({A:Pow(state). F: A leadsTo B})"
 
 syntax (xsymbols)
-  "op leadsTo" :: "[i, i] => i" (infixl "\\<longmapsto>" 60)
+  "leadsTo" :: "[i, i] => i" (infixl "\<longmapsto>" 60)
+
+(** Ad-hoc set-theory rules **)
+
+lemma Int_Union_Union: "Union(B) Int A = (\<Union>b \<in> B. b Int A)"
+by auto
+
+lemma Int_Union_Union2: "A Int Union(B) = (\<Union>b \<in> B. A Int b)"
+by auto
+
+(*** transient ***)
+
+lemma transient_type: "transient(A)<=program"
+by (unfold transient_def, auto)
+
+lemma transientD2: 
+"F \<in> transient(A) ==> F \<in> program & st_set(A)"
+apply (unfold transient_def, auto)
+done
+
+lemma stable_transient_empty: "[| F \<in> stable(A); F \<in> transient(A) |] ==> A = 0"
+by (simp add: stable_def constrains_def transient_def, fast)
+
+lemma transient_strengthen: "[|F \<in> transient(A); B<=A|] ==> F \<in> transient(B)"
+apply (simp add: transient_def st_set_def, clarify)
+apply (blast intro!: rev_bexI)
+done
+
+lemma transientI: 
+"[|act \<in> Acts(F); A <= domain(act); act``A <= state-A;  
+    F \<in> program; st_set(A)|] ==> F \<in> transient(A)"
+by (simp add: transient_def, blast)
+
+lemma transientE: 
+     "[| F \<in> transient(A);  
+         !!act. [| act \<in> Acts(F);  A <= domain(act); act``A <= state-A|]==>P|]
+      ==>P"
+by (simp add: transient_def, blast)
+
+lemma transient_state: "transient(state) = 0"
+apply (simp add: transient_def)
+apply (rule equalityI, auto) 
+apply (cut_tac F = x in Acts_type)
+apply (simp add: Diff_cancel)
+apply (auto intro: st0_in_state)
+done
+
+lemma transient_state2: "state<=B ==> transient(B) = 0"
+apply (simp add: transient_def st_set_def)
+apply (rule equalityI, auto)
+apply (cut_tac F = x in Acts_type)
+apply (subgoal_tac "B=state")
+apply (auto intro: st0_in_state)
+done
+
+lemma transient_empty: "transient(0) = program"
+by (auto simp add: transient_def)
+
+declare transient_empty [simp] transient_state [simp] transient_state2 [simp]
+
+(*** ensures ***)
+
+lemma ensures_type: "A ensures B <=program"
+by (simp add: ensures_def constrains_def, auto)
+
+lemma ensuresI: 
+"[|F:(A-B) co (A Un B); F \<in> transient(A-B)|]==>F \<in> A ensures B"
+apply (unfold ensures_def)
+apply (auto simp add: transient_type [THEN subsetD])
+done
+
+(* Added by Sidi, from Misra's notes, Progress chapter, exercise 4 *)
+lemma ensuresI2: "[| F \<in> A co A Un B; F \<in> transient(A) |] ==> F \<in> A ensures B"
+apply (drule_tac B = "A-B" in constrains_weaken_L)
+apply (drule_tac [2] B = "A-B" in transient_strengthen)
+apply (auto simp add: ensures_def transient_type [THEN subsetD])
+done
+
+lemma ensuresD: "F \<in> A ensures B ==> F:(A-B) co (A Un B) & F \<in> transient (A-B)"
+by (unfold ensures_def, auto)
+
+lemma ensures_weaken_R: "[|F \<in> A ensures A'; A'<=B' |] ==> F \<in> A ensures B'"
+apply (unfold ensures_def)
+apply (blast intro: transient_strengthen constrains_weaken)
+done
+
+(*The L-version (precondition strengthening) fails, but we have this*) 
+lemma stable_ensures_Int: 
+     "[| F \<in> stable(C);  F \<in> A ensures B |] ==> F:(C Int A) ensures (C Int B)"
+ 
+apply (unfold ensures_def)
+apply (simp (no_asm) add: Int_Un_distrib [symmetric] Diff_Int_distrib [symmetric])
+apply (blast intro: transient_strengthen stable_constrains_Int constrains_weaken)
+done
+
+lemma stable_transient_ensures: "[|F \<in> stable(A);  F \<in> transient(C); A<=B Un C|] ==> F \<in> A ensures B"
+apply (frule stable_type [THEN subsetD])
+apply (simp add: ensures_def stable_def)
+apply (blast intro: transient_strengthen constrains_weaken)
+done
+
+lemma ensures_eq: "(A ensures B) = (A unless B) Int transient (A-B)"
+by (auto simp add: ensures_def unless_def)
+
+lemma subset_imp_ensures: "[| F \<in> program; A<=B  |] ==> F \<in> A ensures B"
+by (auto simp add: ensures_def constrains_def transient_def st_set_def)
+
+(*** leadsTo ***)
+lemmas leads_left = leads.dom_subset [THEN subsetD, THEN SigmaD1]
+lemmas leads_right = leads.dom_subset [THEN subsetD, THEN SigmaD2]
+
+lemma leadsTo_type: "A leadsTo B <= program"
+by (unfold leadsTo_def, auto)
+
+lemma leadsToD2: 
+"F \<in> A leadsTo B ==> F \<in> program & st_set(A) & st_set(B)"
+apply (unfold leadsTo_def st_set_def)
+apply (blast dest: leads_left leads_right)
+done
+
+lemma leadsTo_Basis: 
+    "[|F \<in> A ensures B; st_set(A); st_set(B)|] ==> F \<in> A leadsTo B"
+apply (unfold leadsTo_def st_set_def)
+apply (cut_tac ensures_type)
+apply (auto intro: leads.Basis)
+done
+declare leadsTo_Basis [intro]
+
+(* Added by Sidi, from Misra's notes, Progress chapter, exercise number 4 *)
+(* [| F \<in> program; A<=B;  st_set(A); st_set(B) |] ==> A leadsTo B *)
+lemmas subset_imp_leadsTo = subset_imp_ensures [THEN leadsTo_Basis, standard]
+
+lemma leadsTo_Trans: "[|F \<in> A leadsTo B;  F \<in> B leadsTo C |]==>F \<in> A leadsTo C"
+apply (unfold leadsTo_def)
+apply (auto intro: leads.Trans)
+done
+
+(* Better when used in association with leadsTo_weaken_R *)
+lemma transient_imp_leadsTo: "F \<in> transient(A) ==> F \<in> A leadsTo (state-A)"
+apply (unfold transient_def)
+apply (blast intro: ensuresI [THEN leadsTo_Basis] constrains_weaken transientI)
+done
+
+(*Useful with cancellation, disjunction*)
+lemma leadsTo_Un_duplicate: "F \<in> A leadsTo (A' Un A') ==> F \<in> A leadsTo A'"
+by simp
+
+lemma leadsTo_Un_duplicate2:
+     "F \<in> A leadsTo (A' Un C Un C) ==> F \<in> A leadsTo (A' Un C)"
+by (simp add: Un_ac)
+
+(*The Union introduction rule as we should have liked to state it*)
+lemma leadsTo_Union: 
+    "[|!!A. A \<in> S ==> F \<in> A leadsTo B; F \<in> program; st_set(B)|]
+     ==> F \<in> Union(S) leadsTo B"
+apply (unfold leadsTo_def st_set_def)
+apply (blast intro: leads.Union dest: leads_left)
+done
+
+lemma leadsTo_Union_Int: 
+    "[|!!A. A \<in> S ==>F : (A Int C) leadsTo B; F \<in> program; st_set(B)|]  
+     ==> F : (Union(S)Int C)leadsTo B"
+apply (unfold leadsTo_def st_set_def)
+apply (simp only: Int_Union_Union)
+apply (blast dest: leads_left intro: leads.Union)
+done
+
+lemma leadsTo_UN: 
+    "[| !!i. i \<in> I ==> F \<in> A(i) leadsTo B; F \<in> program; st_set(B)|]
+     ==> F:(\<Union>i \<in> I. A(i)) leadsTo B"
+apply (simp add: Int_Union_Union leadsTo_def st_set_def)
+apply (blast dest: leads_left intro: leads.Union)
+done
+
+(* Binary union introduction rule *)
+lemma leadsTo_Un:
+     "[| F \<in> A leadsTo C; F \<in> B leadsTo C |] ==> F \<in> (A Un B) leadsTo C"
+apply (subst Un_eq_Union)
+apply (blast intro: leadsTo_Union dest: leadsToD2)
+done
+
+lemma single_leadsTo_I:
+    "[|!!x. x \<in> A==> F:{x} leadsTo B; F \<in> program; st_set(B) |] 
+     ==> F \<in> A leadsTo B"
+apply (rule_tac b = A in UN_singleton [THEN subst])
+apply (rule leadsTo_UN, auto) 
+done
+
+lemma leadsTo_refl: "[| F \<in> program; st_set(A) |] ==> F \<in> A leadsTo A"
+by (blast intro: subset_imp_leadsTo)
+
+lemma leadsTo_refl_iff: "F \<in> A leadsTo A <-> F \<in> program & st_set(A)"
+by (auto intro: leadsTo_refl dest: leadsToD2)
+
+lemma empty_leadsTo: "F \<in> 0 leadsTo B <-> (F \<in> program & st_set(B))"
+by (auto intro: subset_imp_leadsTo dest: leadsToD2)
+declare empty_leadsTo [iff]
+
+lemma leadsTo_state: "F \<in> A leadsTo state <-> (F \<in> program & st_set(A))"
+by (auto intro: subset_imp_leadsTo dest: leadsToD2 st_setD)
+declare leadsTo_state [iff]
+
+lemma leadsTo_weaken_R: "[| F \<in> A leadsTo A'; A'<=B'; st_set(B') |] ==> F \<in> A leadsTo B'"
+by (blast dest: leadsToD2 intro: subset_imp_leadsTo leadsTo_Trans)
+
+lemma leadsTo_weaken_L: "[| F \<in> A leadsTo A'; B<=A |] ==> F \<in> B leadsTo A'"
+apply (frule leadsToD2)
+apply (blast intro: leadsTo_Trans subset_imp_leadsTo st_set_subset)
+done
+
+lemma leadsTo_weaken: "[| F \<in> A leadsTo A'; B<=A; A'<=B'; st_set(B')|]==> F \<in> B leadsTo B'"
+apply (frule leadsToD2)
+apply (blast intro: leadsTo_weaken_R leadsTo_weaken_L leadsTo_Trans leadsTo_refl)
+done
+
+(* This rule has a nicer conclusion *)
+lemma transient_imp_leadsTo2: "[| F \<in> transient(A); state-A<=B; st_set(B)|] ==> F \<in> A leadsTo B"
+apply (frule transientD2)
+apply (rule leadsTo_weaken_R)
+apply (auto simp add: transient_imp_leadsTo)
+done
+
+(*Distributes over binary unions*)
+lemma leadsTo_Un_distrib: "F:(A Un B) leadsTo C  <->  (F \<in> A leadsTo C & F \<in> B leadsTo C)"
+by (blast intro: leadsTo_Un leadsTo_weaken_L)
+
+lemma leadsTo_UN_distrib: 
+"(F:(\<Union>i \<in> I. A(i)) leadsTo B)<-> ((\<forall>i \<in> I. F \<in> A(i) leadsTo B) & F \<in> program & st_set(B))"
+apply (blast dest: leadsToD2 intro: leadsTo_UN leadsTo_weaken_L)
+done
+
+lemma leadsTo_Union_distrib: "(F \<in> Union(S) leadsTo B) <->  (\<forall>A \<in> S. F \<in> A leadsTo B) & F \<in> program & st_set(B)"
+by (blast dest: leadsToD2 intro: leadsTo_Union leadsTo_weaken_L)
+
+text{*Set difference: maybe combine with @{text leadsTo_weaken_L}??*}
+lemma leadsTo_Diff:
+     "[| F: (A-B) leadsTo C; F \<in> B leadsTo C; st_set(C) |]
+      ==> F \<in> A leadsTo C"
+by (blast intro: leadsTo_Un leadsTo_weaken dest: leadsToD2)
+
+lemma leadsTo_UN_UN:
+    "[|!!i. i \<in> I ==> F \<in> A(i) leadsTo A'(i); F \<in> program |]  
+     ==> F: (\<Union>i \<in> I. A(i)) leadsTo (\<Union>i \<in> I. A'(i))"
+apply (rule leadsTo_Union)
+apply (auto intro: leadsTo_weaken_R dest: leadsToD2) 
+done
+
+(*Binary union version*)
+lemma leadsTo_Un_Un: "[| F \<in> A leadsTo A'; F \<in> B leadsTo B' |] ==> F \<in> (A Un B) leadsTo (A' Un B')"
+apply (subgoal_tac "st_set (A) & st_set (A') & st_set (B) & st_set (B') ")
+prefer 2 apply (blast dest: leadsToD2)
+apply (blast intro: leadsTo_Un leadsTo_weaken_R)
+done
+
+(** The cancellation law **)
+lemma leadsTo_cancel2: "[|F \<in> A leadsTo (A' Un B); F \<in> B leadsTo B'|] ==> F \<in> A leadsTo (A' Un B')"
+apply (subgoal_tac "st_set (A) & st_set (A') & st_set (B) & st_set (B') &F \<in> program")
+prefer 2 apply (blast dest: leadsToD2)
+apply (blast intro: leadsTo_Trans leadsTo_Un_Un leadsTo_refl)
+done
+
+lemma leadsTo_cancel_Diff2: "[|F \<in> A leadsTo (A' Un B); F \<in> (B-A') leadsTo B'|]==> F \<in> A leadsTo (A' Un B')"
+apply (rule leadsTo_cancel2)
+prefer 2 apply assumption
+apply (blast dest: leadsToD2 intro: leadsTo_weaken_R)
+done
+
+
+lemma leadsTo_cancel1: "[| F \<in> A leadsTo (B Un A'); F \<in> B leadsTo B' |] ==> F \<in> A leadsTo (B' Un A')"
+apply (simp add: Un_commute)
+apply (blast intro!: leadsTo_cancel2)
+done
+
+lemma leadsTo_cancel_Diff1:
+     "[|F \<in> A leadsTo (B Un A'); F: (B-A') leadsTo B'|]==> F \<in> A leadsTo (B' Un A')"
+apply (rule leadsTo_cancel1)
+prefer 2 apply assumption
+apply (blast intro: leadsTo_weaken_R dest: leadsToD2)
+done
+
+(*The INDUCTION rule as we should have liked to state it*)
+lemma leadsTo_induct:
+  assumes major: "F \<in> za leadsTo zb"
+      and basis: "!!A B. [|F \<in> A ensures B; st_set(A); st_set(B)|] ==> P(A,B)"
+      and trans: "!!A B C. [| F \<in> A leadsTo B; P(A, B);  
+                              F \<in> B leadsTo C; P(B, C) |] ==> P(A,C)"
+      and union: "!!B S. [| \<forall>A \<in> S. F \<in> A leadsTo B; \<forall>A \<in> S. P(A,B); 
+                           st_set(B); \<forall>A \<in> S. st_set(A)|] ==> P(Union(S), B)"
+  shows "P(za, zb)"
+apply (cut_tac major)
+apply (unfold leadsTo_def, clarify) 
+apply (erule leads.induct) 
+  apply (blast intro: basis [unfolded st_set_def])
+ apply (blast intro: trans [unfolded leadsTo_def]) 
+apply (force intro: union [unfolded st_set_def leadsTo_def]) 
+done
+
+
+(* Added by Sidi, an induction rule without ensures *)
+lemma leadsTo_induct2:
+  assumes major: "F \<in> za leadsTo zb"
+      and basis1: "!!A B. [| A<=B; st_set(B) |] ==> P(A, B)"
+      and basis2: "!!A B. [| F \<in> A co A Un B; F \<in> transient(A); st_set(B) |] 
+                          ==> P(A, B)"
+      and trans: "!!A B C. [| F \<in> A leadsTo B; P(A, B);  
+                              F \<in> B leadsTo C; P(B, C) |] ==> P(A,C)"
+      and union: "!!B S. [| \<forall>A \<in> S. F \<in> A leadsTo B; \<forall>A \<in> S. P(A,B); 
+                           st_set(B); \<forall>A \<in> S. st_set(A)|] ==> P(Union(S), B)"
+  shows "P(za, zb)"
+apply (cut_tac major)
+apply (erule leadsTo_induct)
+apply (auto intro: trans union)
+apply (simp add: ensures_def, clarify)
+apply (frule constrainsD2)
+apply (drule_tac B' = " (A-B) Un B" in constrains_weaken_R)
+apply blast
+apply (frule ensuresI2 [THEN leadsTo_Basis])
+apply (drule_tac [4] basis2, simp_all)
+apply (frule_tac A1 = A and B = B in Int_lower2 [THEN basis1])
+apply (subgoal_tac "A=Union ({A - B, A Int B}) ")
+prefer 2 apply blast
+apply (erule ssubst)
+apply (rule union)
+apply (auto intro: subset_imp_leadsTo)
+done
+
+
+(** Variant induction rule: on the preconditions for B **)
+(*Lemma is the weak version: can't see how to do it in one step*)
+lemma leadsTo_induct_pre_aux: 
+  "[| F \<in> za leadsTo zb;   
+      P(zb);  
+      !!A B. [| F \<in> A ensures B;  P(B); st_set(A); st_set(B) |] ==> P(A);  
+      !!S. [| \<forall>A \<in> S. P(A); \<forall>A \<in> S. st_set(A) |] ==> P(Union(S))  
+   |] ==> P(za)"
+txt{*by induction on this formula*}
+apply (subgoal_tac "P (zb) --> P (za) ")
+txt{*now solve first subgoal: this formula is sufficient*}
+apply (blast intro: leadsTo_refl)
+apply (erule leadsTo_induct)
+apply (blast+)
+done
+
+
+lemma leadsTo_induct_pre: 
+  "[| F \<in> za leadsTo zb;   
+      P(zb);  
+      !!A B. [| F \<in> A ensures B;  F \<in> B leadsTo zb;  P(B); st_set(A) |] ==> P(A);  
+      !!S. \<forall>A \<in> S. F \<in> A leadsTo zb & P(A) & st_set(A) ==> P(Union(S))  
+   |] ==> P(za)"
+apply (subgoal_tac " (F \<in> za leadsTo zb) & P (za) ")
+apply (erule conjunct2)
+apply (frule leadsToD2) 
+apply (erule leadsTo_induct_pre_aux)
+prefer 3 apply (blast dest: leadsToD2 intro: leadsTo_Union)
+prefer 2 apply (blast intro: leadsTo_Trans leadsTo_Basis)
+apply (blast intro: leadsTo_refl)
+done
+
+(** The impossibility law **)
+lemma leadsTo_empty: 
+   "F \<in> A leadsTo 0 ==> A=0"
+apply (erule leadsTo_induct_pre)
+apply (auto simp add: ensures_def constrains_def transient_def st_set_def)
+apply (drule bspec, assumption)+
+apply blast
+done
+declare leadsTo_empty [simp]
+
+subsection{*PSP: Progress-Safety-Progress*}
+
+text{*Special case of PSP: Misra's "stable conjunction"*}
+
+lemma psp_stable: 
+   "[| F \<in> A leadsTo A'; F \<in> stable(B) |] ==> F:(A Int B) leadsTo (A' Int B)"
+apply (unfold stable_def)
+apply (frule leadsToD2) 
+apply (erule leadsTo_induct)
+prefer 3 apply (blast intro: leadsTo_Union_Int)
+prefer 2 apply (blast intro: leadsTo_Trans)
+apply (rule leadsTo_Basis)
+apply (simp add: ensures_def Diff_Int_distrib2 [symmetric] Int_Un_distrib2 [symmetric])
+apply (auto intro: transient_strengthen constrains_Int)
+done
+
+
+lemma psp_stable2: "[|F \<in> A leadsTo A'; F \<in> stable(B) |]==>F: (B Int A) leadsTo (B Int A')"
+apply (simp (no_asm_simp) add: psp_stable Int_ac)
+done
+
+lemma psp_ensures: 
+"[| F \<in> A ensures A'; F \<in> B co B' |]==> F: (A Int B') ensures ((A' Int B) Un (B' - B))"
+apply (unfold ensures_def constrains_def st_set_def)
+(*speeds up the proof*)
+apply clarify
+apply (blast intro: transient_strengthen)
+done
+
+lemma psp: 
+"[|F \<in> A leadsTo A'; F \<in> B co B'; st_set(B')|]==> F:(A Int B') leadsTo ((A' Int B) Un (B' - B))"
+apply (subgoal_tac "F \<in> program & st_set (A) & st_set (A') & st_set (B) ")
+prefer 2 apply (blast dest!: constrainsD2 leadsToD2)
+apply (erule leadsTo_induct)
+prefer 3 apply (blast intro: leadsTo_Union_Int)
+ txt{*Basis case*}
+ apply (blast intro: psp_ensures leadsTo_Basis)
+txt{*Transitivity case has a delicate argument involving "cancellation"*}
+apply (rule leadsTo_Un_duplicate2)
+apply (erule leadsTo_cancel_Diff1)
+apply (simp add: Int_Diff Diff_triv)
+apply (blast intro: leadsTo_weaken_L dest: constrains_imp_subset)
+done
+
+
+lemma psp2: "[| F \<in> A leadsTo A'; F \<in> B co B'; st_set(B') |]  
+    ==> F \<in> (B' Int A) leadsTo ((B Int A') Un (B' - B))"
+by (simp (no_asm_simp) add: psp Int_ac)
+
+lemma psp_unless: 
+   "[| F \<in> A leadsTo A';  F \<in> B unless B'; st_set(B); st_set(B') |]  
+    ==> F \<in> (A Int B) leadsTo ((A' Int B) Un B')"
+apply (unfold unless_def)
+apply (subgoal_tac "st_set (A) &st_set (A') ")
+prefer 2 apply (blast dest: leadsToD2)
+apply (drule psp, assumption, blast)
+apply (blast intro: leadsTo_weaken)
+done
+
+
+subsection{*Proving the induction rules*}
+
+(** The most general rule \<in> r is any wf relation; f is any variant function **)
+lemma leadsTo_wf_induct_aux: "[| wf(r);  
+         m \<in> I;  
+         field(r)<=I;  
+         F \<in> program; st_set(B); 
+         \<forall>m \<in> I. F \<in> (A Int f-``{m}) leadsTo                      
+                    ((A Int f-``(converse(r)``{m})) Un B) |]  
+      ==> F \<in> (A Int f-``{m}) leadsTo B"
+apply (erule_tac a = m in wf_induct2, simp_all)
+apply (subgoal_tac "F \<in> (A Int (f-`` (converse (r) ``{x}))) leadsTo B")
+ apply (blast intro: leadsTo_cancel1 leadsTo_Un_duplicate)
+apply (subst vimage_eq_UN)
+apply (simp del: UN_simps add: Int_UN_distrib)
+apply (auto intro: leadsTo_UN simp del: UN_simps simp add: Int_UN_distrib)
+done
+
+(** Meta or object quantifier ? **)
+lemma leadsTo_wf_induct: "[| wf(r);  
+         field(r)<=I;  
+         A<=f-``I;  
+         F \<in> program; st_set(A); st_set(B);  
+         \<forall>m \<in> I. F \<in> (A Int f-``{m}) leadsTo                      
+                    ((A Int f-``(converse(r)``{m})) Un B) |]  
+      ==> F \<in> A leadsTo B"
+apply (rule_tac b = A in subst)
+ defer 1
+ apply (rule_tac I = I in leadsTo_UN)
+ apply (erule_tac I = I in leadsTo_wf_induct_aux, assumption+, best) 
+done
+
+lemma nat_measure_field: "field(measure(nat, %x. x)) = nat"
+apply (unfold field_def)
+apply (simp add: measure_def)
+apply (rule equalityI, force, clarify)
+apply (erule_tac V = "x\<notin>range (?y) " in thin_rl)
+apply (erule nat_induct)
+apply (rule_tac [2] b = "succ (succ (xa))" in domainI)
+apply (rule_tac b = "succ (0) " in domainI)
+apply simp_all
+done
+
+
+lemma Image_inverse_lessThan: "k<A ==> measure(A, %x. x) -`` {k} = k"
+apply (rule equalityI)
+apply (auto simp add: measure_def)
+apply (blast intro: ltD)
+apply (rule vimageI)
+prefer 2 apply blast
+apply (simp add: lt_Ord lt_Ord2 Ord_mem_iff_lt)
+apply (blast intro: lt_trans)
+done
+
+(*Alternative proof is via the lemma F \<in> (A Int f-`(lessThan m)) leadsTo B*)
+lemma lessThan_induct: 
+ "[| A<=f-``nat;  
+     F \<in> program; st_set(A); st_set(B);  
+     \<forall>m \<in> nat. F:(A Int f-``{m}) leadsTo ((A Int f -`` m) Un B) |]  
+      ==> F \<in> A leadsTo B"
+apply (rule_tac A1 = nat and f1 = "%x. x" in wf_measure [THEN leadsTo_wf_induct]) 
+apply (simp_all add: nat_measure_field)
+apply (simp add: ltI Image_inverse_lessThan vimage_def [symmetric])
+done
+
+
+(*** wlt ****)
+
+(*Misra's property W3*)
+lemma wlt_type: "wlt(F,B) <=state"
+by (unfold wlt_def, auto)
+
+lemma wlt_st_set: "st_set(wlt(F, B))"
+apply (unfold st_set_def)
+apply (rule wlt_type)
+done
+declare wlt_st_set [iff]
+
+lemma wlt_leadsTo_iff: "F \<in> wlt(F, B) leadsTo B <-> (F \<in> program & st_set(B))"
+apply (unfold wlt_def)
+apply (blast dest: leadsToD2 intro!: leadsTo_Union)
+done
+
+(* [| F \<in> program;  st_set(B) |] ==> F \<in> wlt(F, B) leadsTo B  *)
+lemmas wlt_leadsTo = conjI [THEN wlt_leadsTo_iff [THEN iffD2], standard]
+
+lemma leadsTo_subset: "F \<in> A leadsTo B ==> A <= wlt(F, B)"
+apply (unfold wlt_def)
+apply (frule leadsToD2)
+apply (auto simp add: st_set_def)
+done
+
+(*Misra's property W2*)
+lemma leadsTo_eq_subset_wlt: "F \<in> A leadsTo B <-> (A <= wlt(F,B) & F \<in> program & st_set(B))"
+apply auto
+apply (blast dest: leadsToD2 leadsTo_subset intro: leadsTo_weaken_L wlt_leadsTo)+
+done
+
+(*Misra's property W4*)
+lemma wlt_increasing: "[| F \<in> program; st_set(B) |] ==> B <= wlt(F,B)"
+apply (rule leadsTo_subset)
+apply (simp (no_asm_simp) add: leadsTo_eq_subset_wlt [THEN iff_sym] subset_imp_leadsTo)
+done
+
+(*Used in the Trans case below*)
+lemma leadsTo_123_aux: 
+   "[| B <= A2;  
+       F \<in> (A1 - B) co (A1 Un B);  
+       F \<in> (A2 - C) co (A2 Un C) |]  
+    ==> F \<in> (A1 Un A2 - C) co (A1 Un A2 Un C)"
+apply (unfold constrains_def st_set_def, blast)
+done
+
+(*Lemma (1,2,3) of Misra's draft book, Chapter 4, "Progress"*)
+(* slightly different from the HOL one \<in> B here is bounded *)
+lemma leadsTo_123: "F \<in> A leadsTo A'  
+      ==> \<exists>B \<in> Pow(state). A<=B & F \<in> B leadsTo A' & F \<in> (B-A') co (B Un A')"
+apply (frule leadsToD2)
+apply (erule leadsTo_induct)
+  txt{*Basis*}
+  apply (blast dest: ensuresD constrainsD2 st_setD)
+ txt{*Trans*}
+ apply clarify
+ apply (rule_tac x = "Ba Un Bb" in bexI)
+ apply (blast intro: leadsTo_123_aux leadsTo_Un_Un leadsTo_cancel1 leadsTo_Un_duplicate, blast)
+txt{*Union*}
+apply (clarify dest!: ball_conj_distrib [THEN iffD1])
+apply (subgoal_tac "\<exists>y. y \<in> Pi (S, %A. {Ba \<in> Pow (state) . A<=Ba & F \<in> Ba leadsTo B & F \<in> Ba - B co Ba Un B}) ")
+defer 1
+apply (rule AC_ball_Pi, safe)
+apply (rotate_tac 1)
+apply (drule_tac x = x in bspec, blast, blast) 
+apply (rule_tac x = "\<Union>A \<in> S. y`A" in bexI, safe)
+apply (rule_tac [3] I1 = S in constrains_UN [THEN constrains_weaken])
+apply (rule_tac [2] leadsTo_Union)
+prefer 5 apply (blast dest!: apply_type, simp_all)
+apply (force dest!: apply_type)+
+done
+
+
+(*Misra's property W5*)
+lemma wlt_constrains_wlt: "[| F \<in> program; st_set(B) |] ==>F \<in> (wlt(F, B) - B) co (wlt(F,B))"
+apply (cut_tac F = F in wlt_leadsTo [THEN leadsTo_123], assumption, blast)
+apply clarify
+apply (subgoal_tac "Ba = wlt (F,B) ")
+prefer 2 apply (blast dest: leadsTo_eq_subset_wlt [THEN iffD1], clarify)
+apply (simp add: wlt_increasing [THEN subset_Un_iff2 [THEN iffD1]])
+done
+
+
+subsection{*Completion: Binary and General Finite versions*}
+
+lemma completion_aux: "[| W = wlt(F, (B' Un C));      
+       F \<in> A leadsTo (A' Un C);  F \<in> A' co (A' Un C);    
+       F \<in> B leadsTo (B' Un C);  F \<in> B' co (B' Un C) |]  
+    ==> F \<in> (A Int B) leadsTo ((A' Int B') Un C)"
+apply (subgoal_tac "st_set (C) &st_set (W) &st_set (W-C) &st_set (A') &st_set (A) & st_set (B) & st_set (B') & F \<in> program")
+ prefer 2 
+ apply simp 
+ apply (blast dest!: leadsToD2)
+apply (subgoal_tac "F \<in> (W-C) co (W Un B' Un C) ")
+ prefer 2
+ apply (blast intro!: constrains_weaken [OF constrains_Un [OF _ wlt_constrains_wlt]])
+apply (subgoal_tac "F \<in> (W-C) co W")
+ prefer 2
+ apply (simp add: wlt_increasing [THEN subset_Un_iff2 [THEN iffD1]] Un_assoc)
+apply (subgoal_tac "F \<in> (A Int W - C) leadsTo (A' Int W Un C) ")
+ prefer 2 apply (blast intro: wlt_leadsTo psp [THEN leadsTo_weaken])
+(** step 13 **)
+apply (subgoal_tac "F \<in> (A' Int W Un C) leadsTo (A' Int B' Un C) ")
+apply (drule leadsTo_Diff)
+apply (blast intro: subset_imp_leadsTo dest: leadsToD2 constrainsD2)
+apply (force simp add: st_set_def)
+apply (subgoal_tac "A Int B <= A Int W")
+prefer 2 apply (blast dest!: leadsTo_subset intro!: subset_refl [THEN Int_mono])
+apply (blast intro: leadsTo_Trans subset_imp_leadsTo)
+txt{*last subgoal*}
+apply (rule_tac leadsTo_Un_duplicate2)
+apply (rule_tac leadsTo_Un_Un)
+ prefer 2 apply (blast intro: leadsTo_refl)
+apply (rule_tac A'1 = "B' Un C" in wlt_leadsTo[THEN psp2, THEN leadsTo_weaken])
+apply blast+
+done
+
+lemmas completion = refl [THEN completion_aux, standard]
+
+lemma finite_completion_aux:
+     "[| I \<in> Fin(X); F \<in> program; st_set(C) |] ==>  
+       (\<forall>i \<in> I. F \<in> (A(i)) leadsTo (A'(i) Un C)) -->   
+                     (\<forall>i \<in> I. F \<in> (A'(i)) co (A'(i) Un C)) -->  
+                   F \<in> (\<Inter>i \<in> I. A(i)) leadsTo ((\<Inter>i \<in> I. A'(i)) Un C)"
+apply (erule Fin_induct)
+apply (auto simp add: Inter_0)
+apply (rule completion)
+apply (auto simp del: INT_simps simp add: INT_extend_simps)
+apply (blast intro: constrains_INT)
+done
+
+lemma finite_completion: 
+     "[| I \<in> Fin(X);   
+         !!i. i \<in> I ==> F \<in> A(i) leadsTo (A'(i) Un C);  
+         !!i. i \<in> I ==> F \<in> A'(i) co (A'(i) Un C); F \<in> program; st_set(C)|]    
+      ==> F \<in> (\<Inter>i \<in> I. A(i)) leadsTo ((\<Inter>i \<in> I. A'(i)) Un C)"
+by (blast intro: finite_completion_aux [THEN mp, THEN mp])
+
+lemma stable_completion: 
+     "[| F \<in> A leadsTo A';  F \<in> stable(A');    
+         F \<in> B leadsTo B';  F \<in> stable(B') |]  
+    ==> F \<in> (A Int B) leadsTo (A' Int B')"
+apply (unfold stable_def)
+apply (rule_tac C1 = 0 in completion [THEN leadsTo_weaken_R], simp+)
+apply (blast dest: leadsToD2)
+done
+
+
+lemma finite_stable_completion: 
+     "[| I \<in> Fin(X);  
+         (!!i. i \<in> I ==> F \<in> A(i) leadsTo A'(i));  
+         (!!i. i \<in> I ==> F \<in> stable(A'(i)));  F \<in> program |]  
+      ==> F \<in> (\<Inter>i \<in> I. A(i)) leadsTo (\<Inter>i \<in> I. A'(i))"
+apply (unfold stable_def)
+apply (subgoal_tac "st_set (\<Inter>i \<in> I. A' (i))")
+prefer 2 apply (blast dest: leadsToD2)
+apply (rule_tac C1 = 0 in finite_completion [THEN leadsTo_weaken_R], auto) 
+done
+
+ML
+{*
+val Int_Union_Union = thm "Int_Union_Union";
+val Int_Union_Union2 = thm "Int_Union_Union2";
+val transient_type = thm "transient_type";
+val transientD2 = thm "transientD2";
+val stable_transient_empty = thm "stable_transient_empty";
+val transient_strengthen = thm "transient_strengthen";
+val transientI = thm "transientI";
+val transientE = thm "transientE";
+val transient_state = thm "transient_state";
+val transient_state2 = thm "transient_state2";
+val transient_empty = thm "transient_empty";
+val ensures_type = thm "ensures_type";
+val ensuresI = thm "ensuresI";
+val ensuresI2 = thm "ensuresI2";
+val ensuresD = thm "ensuresD";
+val ensures_weaken_R = thm "ensures_weaken_R";
+val stable_ensures_Int = thm "stable_ensures_Int";
+val stable_transient_ensures = thm "stable_transient_ensures";
+val ensures_eq = thm "ensures_eq";
+val subset_imp_ensures = thm "subset_imp_ensures";
+val leads_left = thm "leads_left";
+val leads_right = thm "leads_right";
+val leadsTo_type = thm "leadsTo_type";
+val leadsToD2 = thm "leadsToD2";
+val leadsTo_Basis = thm "leadsTo_Basis";
+val subset_imp_leadsTo = thm "subset_imp_leadsTo";
+val leadsTo_Trans = thm "leadsTo_Trans";
+val transient_imp_leadsTo = thm "transient_imp_leadsTo";
+val leadsTo_Un_duplicate = thm "leadsTo_Un_duplicate";
+val leadsTo_Un_duplicate2 = thm "leadsTo_Un_duplicate2";
+val leadsTo_Union = thm "leadsTo_Union";
+val leadsTo_Union_Int = thm "leadsTo_Union_Int";
+val leadsTo_UN = thm "leadsTo_UN";
+val leadsTo_Un = thm "leadsTo_Un";
+val single_leadsTo_I = thm "single_leadsTo_I";
+val leadsTo_refl = thm "leadsTo_refl";
+val leadsTo_refl_iff = thm "leadsTo_refl_iff";
+val empty_leadsTo = thm "empty_leadsTo";
+val leadsTo_state = thm "leadsTo_state";
+val leadsTo_weaken_R = thm "leadsTo_weaken_R";
+val leadsTo_weaken_L = thm "leadsTo_weaken_L";
+val leadsTo_weaken = thm "leadsTo_weaken";
+val transient_imp_leadsTo2 = thm "transient_imp_leadsTo2";
+val leadsTo_Un_distrib = thm "leadsTo_Un_distrib";
+val leadsTo_UN_distrib = thm "leadsTo_UN_distrib";
+val leadsTo_Union_distrib = thm "leadsTo_Union_distrib";
+val leadsTo_Diff = thm "leadsTo_Diff";
+val leadsTo_UN_UN = thm "leadsTo_UN_UN";
+val leadsTo_Un_Un = thm "leadsTo_Un_Un";
+val leadsTo_cancel2 = thm "leadsTo_cancel2";
+val leadsTo_cancel_Diff2 = thm "leadsTo_cancel_Diff2";
+val leadsTo_cancel1 = thm "leadsTo_cancel1";
+val leadsTo_cancel_Diff1 = thm "leadsTo_cancel_Diff1";
+val leadsTo_induct = thm "leadsTo_induct";
+val leadsTo_induct2 = thm "leadsTo_induct2";
+val leadsTo_induct_pre_aux = thm "leadsTo_induct_pre_aux";
+val leadsTo_induct_pre = thm "leadsTo_induct_pre";
+val leadsTo_empty = thm "leadsTo_empty";
+val psp_stable = thm "psp_stable";
+val psp_stable2 = thm "psp_stable2";
+val psp_ensures = thm "psp_ensures";
+val psp = thm "psp";
+val psp2 = thm "psp2";
+val psp_unless = thm "psp_unless";
+val leadsTo_wf_induct_aux = thm "leadsTo_wf_induct_aux";
+val leadsTo_wf_induct = thm "leadsTo_wf_induct";
+val nat_measure_field = thm "nat_measure_field";
+val Image_inverse_lessThan = thm "Image_inverse_lessThan";
+val lessThan_induct = thm "lessThan_induct";
+val wlt_type = thm "wlt_type";
+val wlt_st_set = thm "wlt_st_set";
+val wlt_leadsTo_iff = thm "wlt_leadsTo_iff";
+val wlt_leadsTo = thm "wlt_leadsTo";
+val leadsTo_subset = thm "leadsTo_subset";
+val leadsTo_eq_subset_wlt = thm "leadsTo_eq_subset_wlt";
+val wlt_increasing = thm "wlt_increasing";
+val leadsTo_123_aux = thm "leadsTo_123_aux";
+val leadsTo_123 = thm "leadsTo_123";
+val wlt_constrains_wlt = thm "wlt_constrains_wlt";
+val completion_aux = thm "completion_aux";
+val completion = thm "completion";
+val finite_completion_aux = thm "finite_completion_aux";
+val finite_completion = thm "finite_completion";
+val stable_completion = thm "stable_completion";
+val finite_stable_completion = thm "finite_stable_completion";
+*}
 
 end
